\documentclass{article}
\usepackage{amsmath}

\begin{document}

\begin{equation}
\rho \left( \frac{\partial \mathbf{v}}{\partial t} + \mathbf{v} \cdot \nabla \mathbf{v} \right) = -\nabla p + \nabla \cdot \mathbf{T} + \mathbf{f}\\
\end{equation}

\begin{equation}
\begin{split}
	\rho \left( \frac{ \partial \mathbf{v} }{ \partial t } + \mathbf{v} \cdot \nabla \mathbf{v} \right) &= - \nabla p + \nabla \cdot \mathbf{T} + \mathbf{f} \\
	1 &= 2
\end{split}
\end{equation}


\begin{align*}
	\rho \left( \frac{ \partial \mathbf{v} }{ \partial t } + \mathbf{v} \cdot \nabla \mathbf{v} \right)  &= - \nabla p + \nabla \cdot \mathbf{T} + \mathbf{f} \\
	\rho \left( \frac{ \partial \mathbf{v} }{ \partial t } + \mathbf{v} \cdot \nabla \mathbf{v} \right) &= - \nabla p + \nabla \cdot \mathbf{T} + \mathbf{f}\\
	1 &= 2
\end{align*}



\end{document}
